Add CheckComparable instruction to make interface equality semantics clearer,
and to avoid using `go_eq : expr` to encode this.

new/golang/defn/postlang.v
@@ -97,22 +97,12 @@ Class GoSemanticsFunctions {ext : ffi_syntax} :=
 
     method_set : go.type → gmap go_string go.signature;
 
-    alloc : go.type → val;
-    load : go.type → val;
-    store : go.type → val;
-
     (* This uses a Gallina [Type] because there are multiple [go.type]s that
        have the same [Type] representation (e.g. uint64/int64, *X/*Y), but
        offsets are only supposed to depend on the Gallina representation. *)
     is_type_repr : go.type → Type → Prop;
     struct_field_ref : Type → go_string → loc → loc;
 
-    (* map index expressions have their own implementation that does not use the
-       `Index` primitive. It's statically (even with type parameters) known
-       whether an index expression is a map index expression or not a map index
-       expression. https://go.dev/ref/spec#Index_expressions *)
-    index (container_type : go.type) (i : Z) (v : val) : expr;
-    index_ref (container_type : go.type) (i : Z) (v : val) : expr;
     array_index_ref (elem_type : Type) (i : Z) (l : loc) : loc;
 
     map_empty : val → val;
@@ -264,7 +254,7 @@ Global Instance is_convert_step from to v from_under to_under v' `{!GoSemanticsF
 Proof. intros. apply is_convert_step_def. Qed.
 
 Class IsGoOp (o : go_operator) (t_under : go.type) v1 v2 e' `{!GoSemanticsFunctions} : Prop :=
-  { is_go_op_step_def `{!t ↓u t_under} :: IsGoStepPureDet (GoOp o t) (v1, v2)%V e' }.
+  { is_go_op_step_def `{!t ↓u t_under} : IsGoStepPureDet (GoOp o t) (v1, v2)%V e' }.
 Global Hint Mode IsGoOp + + + + - - : typeclass_instances.
 Global Instance is_go_op_step o t t_under v1 v2 e' `{!GoSemanticsFunctions} :
   t ↓u t_under → IsGoOp o t_under v1 v2 e' →
@@ -272,12 +262,20 @@ Global Instance is_go_op_step o t t_under v1 v2 e' `{!GoSemanticsFunctions} :
 Proof. intros. apply is_go_op_step_def. Qed.
 
 Class IsCompositeLiteral (t_under : go.type) v e' `{!GoSemanticsFunctions} : Prop :=
-  { is_composite_literal_step_def `{!t ↓u t_under} :: IsGoStepPureDet (CompositeLiteral t) v (e' t) }.
+  { is_composite_literal_step_def `{!t ↓u t_under} : IsGoStepPureDet (CompositeLiteral t) v (e' t) }.
 Global Hint Mode IsCompositeLiteral + + - - : typeclass_instances.
 Global Instance is_composite_literal_step t t_under v e' `{!GoSemanticsFunctions} :
   t ↓u t_under → IsCompositeLiteral t_under v e' →
   IsGoStepPureDet (CompositeLiteral t) v (e' t).
 Proof. intros. apply is_composite_literal_step_def. Qed.
+
+Class IsComparable (t_under : go.type) `{!GoSemanticsFunctions} : Prop :=
+  { is_comparable_check_step_def `{!t ↓u t_under} :: IsGoStepPureDet (CheckComparable t) #() #() }.
+Global Hint Mode IsComparable + - : typeclass_instances.
+Global Instance is_comparable_step t t_under `{!GoSemanticsFunctions} :
+  t ↓u t_under → IsComparable t_under →
+  IsGoStepPureDet (CheckComparable t) #() #().
+Proof. intros. apply is_comparable_check_step_def. Qed.
 
 (* Helper definition to cover types for which `a == b` always executes safely. *)
 Class IsStrictlyComparable t V `{!EqDecision V} `{!GoSemanticsFunctions} : Prop :=
@@ -288,15 +286,22 @@ Class IsStrictlyComparable t V `{!EqDecision V} `{!GoSemanticsFunctions} : Prop 
 
 Class CoreComparisonSemantics `{!GoSemanticsFunctions} : Prop :=
 {
+  #[global] primitive_is_comparable t (H : is_primitive t) :: IsComparable t;
+
   (* special case equality for functions *)
   #[global] is_go_op_go_equals_func_nil_l sig f ::
     IsGoOp GoEquals (go.FunctionType sig) #f #func.nil #(bool_decide (f = func.nil));
   #[global] is_go_op_go_equals_func_nil_r sig f ::
     IsGoOp GoEquals (go.FunctionType sig) #func.nil #f #(bool_decide (f = func.nil));
 
+  #[global] pointer_is_comparable t :: IsComparable (go.PointerType t);
   #[global] go_eq_pointer t :: IsStrictlyComparable (go.PointerType t) loc;
+  #[global] channel_is_comparable dir t :: IsComparable (go.ChannelType dir t);
   #[global] go_eq_channel t dir :: IsStrictlyComparable (go.ChannelType t dir) loc;
 
+  #[global] struct_is_comparable fds
+    `{!TCForall (λ fd, IsComparable (match fd with go.FieldDecl _ t | go.EmbeddedField _ t => t end)) fds} ::
+    IsComparable (go.StructType fds);
   #[global] go_eq_struct fds v1 v2 ::
     IsGoOp GoEquals (go.StructType fds) v1 v2
     (foldl (λ cmp_so_far fd,
@@ -318,6 +323,78 @@ Fixpoint struct_field_type (f : go_string) (fds : list go.field_decl) : go.type 
       else struct_field_type f fds
   end.
 
+Class TypeRepr t V `{!ZeroVal V} `{!GoSemanticsFunctions} : Prop :=
+  {
+    type_repr : is_type_repr t V;
+    #[global] go_zero_val_step :: IsGoStepPureDet (GoZeroVal t) #() #(zero_val V);
+  }.
+Global Hint Mode TypeRepr ! - - - : typeclass_instances.
+
+End defs.
+
+Global Notation "s  ≤u  t" := (go.UnderlyingEq s t) (at level 70).
+Global Notation "s  <u  t" := (go.UnderlyingDirectedEq s t) (at level 70).
+Global Notation "t  ↓u  tunder" := (go.IsUnderlying t tunder) (at level 70).
+
+Module mem.
+Section defs.
+Context {ext : ffi_syntax} {go_lctx : GoLocalContext} {go_gctx : GoGlobalContext}.
+Class MemSemantics `{!GoSemanticsFunctions} : Prop :=
+{
+  #[export] alloc_primitive `[!t ↓u tunder] v (H : is_primitive tunder) ::
+    IsGoStepPureDet (GoAlloc t) v (ref_one v)%E;
+  #[export] alloc_struct `[!t ↓u go.StructType fds] v ::
+    IsGoStepPureDet (GoAlloc t) v
+      (let: "l" := GoPrealloc #() in
+       foldr (λ fd alloc_rest,
+                let (field_name, field_type) := match fd with
+                                                | go.FieldDecl n t => pair n t
+                                                | go.EmbeddedField n t => pair n t
+                                                end in
+                let field_addr := StructFieldRef t field_name "l" in
+                let: "l_field" := GoAlloc field_type (StructFieldGet t field_name v) in
+                (if: ("l_field" ≠⟨go.PointerType field_type⟩ field_addr) then AngelicExit #()
+                 else #());;
+                alloc_rest
+         ) #() fds ;;
+       "l")%E;
+
+  #[export] load_primitive `[!t ↓u tunder] (H : is_primitive tunder) l ::
+    IsGoStepPureDet (GoLoad t) l (Read l)%E;
+
+  #[export] load_struct `[!t ↓u go.StructType fds] l ::
+    IsGoStepPureDet (GoLoad t) l
+      (foldl (λ struct_so_far fd,
+                let (field_name, field_type) := match fd with
+                                                | go.FieldDecl n t => pair n t
+                                                | go.EmbeddedField n t => pair n t
+                                                end in
+                let field_addr := StructFieldRef t field_name l in
+                let field_val := GoLoad field_type field_addr in
+                StructFieldSet t field_name (struct_so_far, field_val)
+         )%E (GoZeroVal t #()) fds)%V;
+
+  #[export] store_primitive `[!t ↓u tunder] (H : is_primitive t) l v ::
+    IsGoStepPureDet (GoStore t) (l, v)%V (l <- v)%E;
+  store_struct `[!t ↓u go.StructType fds] l v :
+    IsGoStepPureDet (GoStore t) (l, v)
+      (foldl (λ store_so_far fd,
+                store_so_far;;
+                let (field_name, field_type) := match fd with
+                                                | go.FieldDecl n t => pair n t
+                                                | go.EmbeddedField n t => pair n t
+                                                end in
+                let field_addr := StructFieldRef t field_name l in
+                let field_val := StructFieldGet t field_name v in
+                GoStore field_type (field_addr, field_val)
+         )%E (#()) fds)%V;
+
+}.
+End defs.
+End mem.
+
+Section defs.
+Context {ext : ffi_syntax} {go_lctx : GoLocalContext} {go_gctx : GoGlobalContext}.
 Class IntoValUnfold V f :=
   {
     into_val_unfold : @into_val _ _ V = f;
@@ -344,14 +421,6 @@ Class BasicIntoValInj :=
     #[global] into_val_inj_interface :: IntoValInj interface.t;
     #[global] into_val_inj_proph_id :: IntoValInj proph_id;
   }.
-
-Class TypeRepr t V `{!ZeroVal V} `{!GoSemanticsFunctions} : Prop :=
-  {
-    type_repr : is_type_repr t V;
-    #[global] go_zero_val_step :: IsGoStepPureDet (GoZeroVal t) #() #(zero_val V);
-  }.
-Global Hint Mode TypeRepr ! - - - : typeclass_instances.
-
 (** [go.CoreSemantics] defines the basics of when a GoContext is valid,
     excluding predeclared types (including primitives), arrays, slice, map, and
     channels, each of which is in their own file. *)
@@ -361,9 +430,6 @@ Class CoreSemantics `{!GoSemanticsFunctions} : Prop :=
 
   #[global] underlying_not_named `{!NotNamed t} :: t ↓u t;
 
-  #[global] go_alloc_step t args :: IsGoStepPureDet (GoAlloc t) args (alloc t args);
-  #[global] go_load_step t (l : loc) :: IsGoStepPureDet (GoLoad t) #l (load t #l);
-  #[global] go_store_step t (l : loc) v :: IsGoStepPureDet (GoStore t) (#l, v)%V (store t #l v);
   #[global] go_func_resolve_step n ts :: IsGoStepPureDet (FuncResolve n ts) #() #(functions n ts);
   #[global] go_method_resolve_step m t rcvr `{!t ↓u tunder} `{!NotInterface tunder} ::
     IsGoStepPureDet (MethodResolve t m) rcvr #(methods t m rcvr);
@@ -405,65 +471,7 @@ Class CoreSemantics `{!GoSemanticsFunctions} : Prop :=
   #[global] type_repr_map key_type elem_type :: TypeRepr (go.MapType key_type elem_type) map.t;
 
   #[global] core_comparison_sem :: CoreComparisonSemantics;
-
-  alloc_underlying `{!t ≤u tunder} : alloc t = alloc tunder;
-  alloc_primitive t (H : is_primitive t) : alloc t = (λ: "v", ref_one "v")%V;
-  alloc_struct `{!t ≤u go.StructType fds} :
-    alloc t =
-    (λ: "v",
-        let: "l" := GoPrealloc #() in
-        foldr (λ fd alloc_rest,
-                 let (field_name, field_type) := match fd with
-                                                 | go.FieldDecl n t => pair n t
-                                                 | go.EmbeddedField n t => pair n t
-                                                 end in
-                 let field_addr := StructFieldRef t field_name "l" in
-                 let: "l_field" := GoAlloc field_type (StructFieldGet t field_name "v") in
-                 (if: ("l_field" ≠⟨go.PointerType field_type⟩ field_addr) then AngelicExit #()
-                  else #());;
-                 alloc_rest
-          ) #() fds ;;
-        "l")%V;
-
-  load_underlying `{!t ≤u tunder} : load t = load tunder;
-  load_primitive t (H : is_primitive t) : load t = (λ: "l", Read "l")%V;
-  load_struct `{!t ≤u go.StructType fds} :
-    load t =
-    (λ: "l",
-       foldl (λ struct_so_far fd,
-                let (field_name, field_type) := match fd with
-                                                | go.FieldDecl n t => pair n t
-                                                | go.EmbeddedField n t => pair n t
-                                                end in
-                let field_addr := StructFieldRef t field_name "l" in
-                let field_val := GoLoad field_type field_addr in
-                StructFieldSet t field_name (struct_so_far, field_val)
-         ) (GoZeroVal t #()) fds)%V;
-
-  store_underlying `{!t ≤u tunder} : store t = store tunder;
-  store_primitive t (H : is_primitive t) : store t = (λ: "l" "v", "l" <- "v")%V;
-  store_struct `{!t ≤u go.StructType fds} :
-    store t =
-    (λ: "l" "v",
-       foldl (λ store_so_far fd,
-                store_so_far;;
-                let (field_name, field_type) := match fd with
-                                                | go.FieldDecl n t => pair n t
-                                                | go.EmbeddedField n t => pair n t
-                                                end in
-                let field_addr := StructFieldRef t field_name "l" in
-                let field_val := StructFieldGet t field_name "v" in
-                GoStore field_type (field_addr, field_val)
-         ) (#()) fds)%V;
-
-  index_ref_underlying `{!t ≤u t'} : index_ref t = index_ref t';
-  index_underlying `{!t ≤u t'} : index t = index t';
-
-  #[global] index_ref_step t (j : w64) (v : val) ::
-    IsGoStepPureDet (IndexRef t) (v, #j)%V (index_ref t (sint.Z j) v);
-
-  #[global] index_step t (j : w64) (v : val) ::
-    IsGoStepPureDet (Index t) (v, #j)%V (index t (sint.Z j) v);
+  #[global] core_mem_sem :: mem.MemSemantics;
 
   #[global] composite_literal_pointer elem_type l ::
     IsCompositeLiteral (go.PointerType elem_type) l
